src/Parsers/Grammars/ABStar.v
@@ -1,0 +1,53 @@
+(** * Definition of grammar for regular expression [(ab)*] *)
+Require Import Coq.Strings.String Coq.Strings.Ascii Coq.Lists.List.
+Require Import Parsers.ContextFreeGrammar Parsers.ContextFreeGrammarNotations.
+
+Set Implicit Arguments.
+
+Section ab_star.
+  Local Open Scope string_scope.
+
+  Definition ab_star_grammar : grammar Ascii.ascii :=
+    {| Start_symbol := "(ab)*";
+       Lookup := [[[ ("(ab)*" ::== << nil
+                                     | $< "a"%char $ "b"%char $ "(ab)*" >$ >> ) ]]]%prods_assignment;
+       Valid_nonterminals := ("(ab)*"::nil)%string |}.
+End ab_star.
+
+Create HintDb cfg discriminated.
+Hint Constructors parse_of parse_of_production parse_of_item : cfg.
+Hint Resolve ParseProductionSingleton ParseProductionApp ParseApp : cfg.
+
+Section tests.
+  Example ab_star_parses_empty : parse_of_grammar string_stringlike (Empty _) ab_star_grammar.
+  Proof.
+    hnf; simpl.
+    repeat constructor.
+  Defined.
+
+  Example ab_star_parses_ab : parse_of_grammar string_stringlike "ab"%string ab_star_grammar.
+  Proof.
+    hnf; simpl.
+    constructor (constructor); simpl.
+    apply ParseProductionCons with (str := "a"%string) (strs := "b"%string).
+    { refine (ParseTerminal _ _ _). }
+    { apply ParseProductionCons with (str := "b"%string) (strs := ""%string).
+      { refine (ParseTerminal _ _ _). }
+      { apply ParseProductionCons with (str := ""%string) (strs := ""%string);
+        repeat (simpl; constructor). } }
+  Defined.
+
+  Example ab_star_parses_abab : parse_of_grammar string_stringlike "abab"%string ab_star_grammar.
+  Proof.
+    hnf; simpl.
+    constructor (constructor); simpl.
+    apply ParseProductionCons with (str := "a"%string) (strs := "bab"%string).
+    { refine (ParseTerminal _ _ _). }
+    { apply ParseProductionCons with (str := "b"%string) (strs := "ab"%string).
+      { refine (ParseTerminal _ _ _). }
+      { apply ParseProductionCons with (str := "ab"%string) (strs := ""%string).
+        { constructor.
+          apply ab_star_parses_ab. }
+        { constructor. } } }
+  Defined.
+End tests.
