src/Parsers/Grammars/Trivial.v
@@ -1,0 +1,32 @@
+(** * Definition of ε, the CFG accepting only "" *)
+Require Import Coq.Strings.String Coq.Lists.List.
+Require Import Parsers.ContextFreeGrammar.
+
+Set Implicit Arguments.
+
+Section generic.
+  Variable CharType : Type.
+  Variable String : string_like CharType.
+
+  Definition trivial_grammar : grammar CharType :=
+    {| Start_symbol := "";
+       Lookup := fun _ => nil::nil;
+       Valid_nonterminals := ""%string::nil |}.
+
+  Definition trivial_grammar_parses_empty_string : parse_of_grammar _ (Empty String) trivial_grammar.
+  Proof.
+    hnf; simpl.
+    apply ParseHead.
+    constructor.
+  Defined.
+
+  Lemma trivial_grammar_parses_only_empty_string s : parse_of_grammar _ s trivial_grammar -> s = Empty String.
+  Proof.
+    intro H; hnf in H; simpl in H.
+    repeat match goal with
+             | _ => reflexivity
+             | [ H : parse_of _ _ _ _ |- _ ] => inversion_clear H
+             | [ H : parse_of_production _ _ _ _ |- _ ] => inversion_clear H
+           end.
+  Qed.
+End generic.
